code/blake2/Hacl.Impl.Blake2.Core.fsti
@@ -17,10 +17,10 @@ type m_spec =
   | M256
 
 inline_for_extraction
-unfold type word_t (a:Spec.alg) = Spec.word_t a
+type word_t (a:Spec.alg) = Spec.word_t a
 
 inline_for_extraction
-unfold let element_t (a:Spec.alg) (m:m_spec) =
+let element_t (a:Spec.alg) (m:m_spec) =
   match a,m with
   | Spec.Blake2S,M128 -> (vec_t U32 4)
   | Spec.Blake2S,M256 -> (vec_t U32 4)
@@ -31,7 +31,13 @@ inline_for_extraction
 val zero_element: a:Spec.alg -> m:m_spec -> element_t a m
 
 inline_for_extraction
-val row_len: a:Spec.alg -> m:m_spec -> size_t
+let row_len (a:Spec.alg) (m:m_spec) : size_t =
+  match a,m with
+  | Spec.Blake2S,M128 -> 1ul
+  | Spec.Blake2S,M256 -> 1ul
+  | Spec.Blake2B,M256 -> 1ul
+  | _ -> 4ul
+
 
 
 inline_for_extraction
@@ -59,7 +65,7 @@ let g_rowi (#a:Spec.alg) (#m:m_spec) (st:state_p a m)  (idx:index_t) : GTot (row
   gsub st (idx *. row_len a m) (row_len a m)
 
 val g_rowi_disjoint: #a:Spec.alg -> #m:m_spec -> st:state_p a m -> idx1:index_t -> idx2:index_t ->
-  Lemma (ensures (idx1 <> idx2 ==> disjoint (g_rowi st idx1) (g_rowi st idx2)))
+  Lemma (ensures (v idx1 <> v idx2 ==> disjoint (g_rowi st idx1) (g_rowi st idx2)))
 	[SMTPat (disjoint (g_rowi st idx1) (g_rowi st idx2))]
 
 val g_rowi_unchanged: #a:Spec.alg -> #m:m_spec -> h0:mem -> h1:mem -> st:state_p a m -> i:index_t ->
@@ -67,22 +73,40 @@ val g_rowi_unchanged: #a:Spec.alg -> #m:m_spec -> h0:mem -> h1:mem -> st:state_p
 	(ensures (as_seq h0 (g_rowi st i) == as_seq h1 (g_rowi st i)))
 	[SMTPat (as_seq h0 (g_rowi st i)); SMTPat (as_seq h1 (g_rowi st i))]
 
-val g_rowi_disjoint_other:  #a:Spec.alg -> #m:m_spec -> #b:Type -> #len:size_t -> st:state_p a m -> i:index_t -> x:lbuffer b len ->
+val g_rowi_disjoint_other:  #a:Spec.alg -> #m:m_spec -> #b:Type -> st:state_p a m -> i:index_t -> x:buffer b ->
   Lemma(requires (disjoint st x))
-       (ensures (disjoint (g_rowi st i) x /\ disjoint x (g_rowi st i)))
-
+       (ensures (disjoint (g_rowi st i) x))
+       [SMTPat (disjoint (g_rowi st i) x)]
 
 inline_for_extraction noextract
 val state_v: #a:Spec.alg -> #m:m_spec -> mem -> state_p a m -> GTot (Spec.state a)
 
 noextract
-val state_v_lemma: #a:Spec.alg -> #m:m_spec -> h0:mem -> h1:mem -> st:state_p a m ->
+val state_v_eq_lemma: #a:Spec.alg -> #m:m_spec -> h0:mem -> h1:mem -> st:state_p a m ->
   Lemma (requires (as_seq h0 st == as_seq h1 st))
 	(ensures (state_v h0 st == state_v h1 st))
-	[SMTPat (state_v h0 st); SMTPat (state_v h1 st)]
+	[SMTPat (state_v #a #m h0 st); SMTPat (state_v #a #m h1 st)]
 
+noextract
+val state_v_rowi_lemma: #a:Spec.alg -> #m:m_spec -> h:mem -> st:state_p a m -> i:index_t ->
+  Lemma (requires (live h st))
+	(ensures (Lib.Sequence.((state_v h st).[v i] == row_v h (g_rowi st i))))
+	[SMTPat (row_v h (g_rowi st i))]
 
-val modifies_row: a:Spec.alg -> m:m_spec -> h0:mem -> h1:mem -> st:state_p a m -> i:index_t ->
+noextract
+val state_v_live_rowi_lemma: #a:Spec.alg -> #m:m_spec -> h:mem -> st:state_p a m -> i:index_t ->
+  Lemma (requires (live h st))
+	(ensures (live h (g_rowi st i)))
+	[SMTPat (live h (g_rowi st i))]
+
+noextract
+val modifies_one_row: a:Spec.alg -> m:m_spec -> h0:mem -> h1:mem -> st:state_p a m -> i:index_t -> j:index_t ->
+  Lemma (requires (live h0 st /\ modifies (loc (g_rowi st i)) h0 h1 /\ v i <> v j))
+	(ensures (row_v h1 (g_rowi st j) == row_v h0 (g_rowi st j)))
+	[SMTPat (modifies (loc (g_rowi st i)) h0 h1); SMTPat (row_v h1 (g_rowi st j))]
+
+noextract
+val modifies_row_state: a:Spec.alg -> m:m_spec -> h0:mem -> h1:mem -> st:state_p a m -> i:index_t ->
   Lemma (requires (live h0 st /\ modifies (loc (g_rowi st i)) h0 h1))
 	(ensures (state_v h1 st == Lib.Sequence.((state_v h0 st).[v i] <- row_v h1 (g_rowi st i))))
 	[SMTPat (modifies (loc (g_rowi st i)) h0 h1)]
@@ -144,12 +168,26 @@ val load_row: #a:Spec.alg -> #m:m_spec -> r1:row_p a m -> ws:lbuffer (word_t a) 
 	  (ensures (fun h0 _ h1 -> modifies (loc r1) h0 h1 /\
 				row_v h1 r1 == Spec.( load_row (as_seq h0 ws))))
 
+
 inline_for_extraction
-val gather_row: #a:Spec.alg -> #ms:m_spec -> #len:size_t -> r:row_p a ms -> m:lbuffer uint8 len ->
-          i0: Spec.word_index a (v len) -> i1:Spec.word_index a (v len) -> i2:Spec.word_index a (v len) -> i3:Spec.word_index a (v len)
+let size_block (a:Spec.alg): x:size_t = size (Spec.size_block a)
+
+inline_for_extraction
+type block_p (a:Spec.alg) = lbuffer uint8 (size_block a)
+
+inline_for_extraction
+val gather_row: #a:Spec.alg -> #ms:m_spec -> r:row_p a ms -> m:block_p a ->
+          i0: Spec.sigma_elt_t -> i1:Spec.sigma_elt_t -> i2:Spec.sigma_elt_t -> i3:Spec.sigma_elt_t
 	  -> ST unit
 	  (requires (fun h -> live h r /\ live h m /\ disjoint r m))
 	  (ensures (fun h0 _ h1 -> modifies (loc r) h0 h1 /\
 				row_v h1 r == Spec.( gather_row (as_seq h0 m) i0 i1 i2 i3)))
 
+
+inline_for_extraction
+val alloc_state: a:Spec.alg -> m:m_spec ->
+	  StackInline (state_p a m)
+	  (requires (fun h -> True))
+	  (ensures (fun h0 r h1 -> stack_allocated r h0 h1 (Lib.Sequence.create (4 * v (row_len a m)) (zero_element a m)) /\
+				live h1 r))
 
